



Neural-Fly Enables Rapid Learning for Agile Flight in Strong Winds

Book/Paper	Control
Field	Control
Contains Formulas	<input type="checkbox"/>
Contains Images	<input type="checkbox"/>

1 Euler–Lagrange dynamics with aerodynamic force + error-based control equation

1.1 Full dynamics (including aerodynamic force)

We consider an Euler–Lagrange (EL) mechanical system with generalized coordinates and velocities:

$$q(t) \in \mathbb{R}^n, \quad \dot{q}(t) \in \mathbb{R}^n.$$

The dynamics (with aerodynamic / disturbance force) are:

$$M(q) \ddot{q} + C(q, \dot{q}) \dot{q} + g(q) = u + f(q, \dot{q}, w),$$

where:

$$M(q) \in \mathbb{R}^{n \times n} \text{ is symmetric positive definite, } C(q, \dot{q}) \in \mathbb{R}^{n \times n}, \quad g(q) \in \mathbb{R}^n.$$

The unknown aerodynamic force is denoted:

$$f(q, \dot{q}, w) \in \mathbb{R}^n,$$

Key EL structural identity

A classical property of EL systems is that: $\dot{M}(q) - 2C(q, \dot{q})$ is skew-symmetric

which implies for any vector $x \in \mathbb{R}^n$

$$x^\top (\dot{M} - 2C) x = 0 \quad \Longleftrightarrow \quad x^\top \dot{M} x = 2x^\top C x.$$

We will use this to simplify the Lyapunov derivative later.

1.2 Tracking errors and the “composite” error variable s

Let $q_d(t)$ be a desired trajectory (at least twice differentiable). Define tracking errors:

$$\tilde{q} := q - q_d, \quad \dot{\tilde{q}} := \dot{q} - \dot{q}_d.$$

Choose a constant gain matrix:

$$\Lambda \in \mathbb{R}^{n \times n}, \quad \Lambda \succ 0.$$

Define the “composite” tracking error:

$$s := \dot{\tilde{q}} + \Lambda \tilde{q}.$$

Define the reference velocity/acceleration (standard in EL control):

$$\dot{q}_r := \dot{q}_d - \Lambda \tilde{q}, \quad \ddot{q}_r := \ddot{q}_d - \Lambda \dot{\tilde{q}}.$$

Then you can verify:

$$s = \dot{q} - \dot{q}_r, \quad \dot{s} = \ddot{q} - \ddot{q}_r.$$

1.3 Aerodynamic force model, estimation, and why parameter-error divergence is dangerous

We assume the unknown aerodynamic force admits a **low-dimensional linear-in-parameters representation** plus a residual:

$$f(q, \dot{q}, w) = \phi(q, \dot{q}) a(t) + d(t).$$

- $\phi(q, \dot{q}) \in \mathbb{R}^{n \times h}$: known "basis/features" (e.g., a neural network output evaluated online)
- $a(t) \in \mathbb{R}^h$: unknown time-varying coefficient (captures wind-dependent effects)
- $d(t) \in \mathbb{R}^n$: unmodeled remainder (representation error, unmodeled physics, etc.)

We maintain an online estimate $\hat{a}(t)$, Define parameter estimation error

$$\tilde{a} = \hat{a} - a.$$

Then the estimated aerodynamic force is:

$$\hat{f} = \phi(q, \dot{q}) \hat{a}.$$

The **force estimation error** becomes:

$$f - \hat{f} = \phi a + d - \phi \hat{a} = -\phi \tilde{a} + d.$$

Why \tilde{a} can destabilize the system

If $\tilde{a}(t)$ is not guaranteed bounded, then the term $-\phi \tilde{a}$ can grow without bound and acts like an **unbounded input** injected into the closed-loop error dynamics. Even if we add stabilizing feedback $-Ks$, an unbounded forcing term can dominate and drive s large, breaking tracking (and potentially saturating actuators in practice).

So: **stability requires controlling both s and \tilde{a}**

1.4 Control law and the closed-loop error equation in s

Choose a feedback gain:

$$K \in \mathbb{R}^{n \times n}, \quad K \succ 0.$$

Define the control input:

$$u = M(q) \ddot{q}_r + C(q, \dot{q}) \dot{q}_r + g(q) - Ks - \phi(q, \dot{q}) \hat{a}.$$

Now derive the s dynamics.

Start from the plant:

$$M\ddot{q} + C\dot{q} + g = u + f.$$

Substitute u and cancel terms:

$$M\ddot{q} + C\dot{q} + g = (M\ddot{q}_r + C\dot{q}_r + g - Ks - \phi \hat{a}) + f.$$

Bring $M\ddot{q}_r + C\dot{q}_r + g$ to the left:

$$M(\ddot{q} - \ddot{q}_r) + C(\dot{q} - \dot{q}_r) = -Ks - \phi\hat{a} + f.$$

Use:

$$\dot{s} = \ddot{q} - \ddot{q}_r, \quad s = \dot{q} - \dot{q}_r,$$

to obtain:

$$M\dot{s} + Cs = -Ks - \phi\hat{a} + f.$$

Replace $f = \phi a + d$, and group $\tilde{a} = \hat{a} - a$

$$M\dot{s} + Cs = -Ks - \phi(\hat{a} - a) + d$$

$$M\dot{s} + (C + K)s = -\phi\tilde{a} + d$$

This is the key “tracking-error dynamics with parameter error injection.

2. Why we introduce a joint Lyapunov function + exponential contraction to an error ball

2.1 If we only use tracking energy, we need \tilde{a} bounded (not automatic)

A natural tracking-only Lyapunov candidate is:

$$V_s := \frac{1}{2} s^\top M(q) s.$$

Its derivative is:

$$\dot{V}_s = s^\top M\dot{s} + \frac{1}{2} s^\top \dot{M}s.$$

Using the closed-loop equation:

$$M\dot{s} = -(C + K)s - \phi\tilde{a} + d,$$

we get:

$$\dot{V}_s = s^\top (-(C + K)s - \phi\tilde{a} + d) + \frac{1}{2} s^\top \dot{M}s = -s^\top Ks + s^\top (d - \phi\tilde{a}) + \left(-s^\top Cs + \frac{1}{2} s^\top \dot{M}s \right).$$

Using EL identity:

$$-s^\top Cs + \frac{1}{2} s^\top \dot{M}s = 0,$$

$$\dot{V}_s = -s^\top Ks + s^\top (d - \phi\tilde{a}).$$

Bounding:

$$s^\top Ks \geq \lambda_{\min}(K) \|s\|^2,$$

$$s^\top (d - \phi\tilde{a}) \leq \|s\| \|d - \phi\tilde{a}\|.$$

$$\dot{V}_s \leq -\lambda_{\min}(K) \|s\|^2 + \|s\| \|d - \phi\tilde{a}\|.$$

This implies “ultimate boundedness” **only if** $\|d - \phi\tilde{a}\|$ is bounded—i.e., you need \tilde{a} bounded. But **boundedness of \tilde{a}** is *not automatic* unless we design an update law for \hat{a} that enforces it.

Hence we introduce a **joint** Lyapunov function including \tilde{a}

2.2 Joint Lyapunov function (tracking + parameter-error energy)

We choose:

$$V := \frac{1}{2} s^\top M s + \frac{1}{2} \tilde{a}^\top P^{-1} \tilde{a},$$

where:

$$P(t) \in \mathbb{R}^{h \times h}, \quad P(t) \succ 0$$

is a time-varying positive definite matrix (later we will define its dynamics).

This is “equivalent energy” because:

- $s^\top M s$ is kinetic-like energy in the tracking error
- $\tilde{a}^\top P^{-1} \tilde{a}$ measures parameter error magnitude under the metric P^{-1}

2.3 Derivative of the joint Lyapunov function and the key coupling term

Compute:

$$\dot{V} = \dot{V}_s + \dot{V}_a,$$

where \dot{V}_s is already known:

$$\dot{V}_s = -s^\top K s + s^\top (d - \phi \tilde{a}).$$

Now handle:

$$V_a := \frac{1}{2} \tilde{a}^\top P^{-1} \tilde{a}.$$

Differentiate (product rule; both \tilde{a} and P^{-1} vary):

$$\begin{aligned} \dot{V}_a &= \tilde{a}^\top P^{-1} \dot{\tilde{a}} + \frac{1}{2} \dot{\tilde{a}}^\top (P^{-1}) \tilde{a}. \\ \dot{V} &= -s^\top K s + s^\top d - s^\top \phi \tilde{a} + \tilde{a}^\top P^{-1} \dot{\tilde{a}} + \frac{1}{2} \dot{\tilde{a}}^\top (P^{-1}) \tilde{a}. \end{aligned}$$

The problematic coupling term is:

$$-s^\top \phi \tilde{a}.$$

To make \dot{V} negative (up to bounded disturbance terms), we want **an opposite term** $+s^\top \phi \tilde{a}$ appear from $\tilde{a}^\top P^{-1} \dot{\tilde{a}}$

This motivates including a **tracking-driven** component in $\dot{\tilde{a}}$ such that:

$$\dot{\tilde{a}} \supset P \phi^\top s.$$

Because then:

$$\tilde{a}^\top P^{-1} (P \phi^\top s) = \tilde{a}^\top \phi^\top s = s^\top \phi \tilde{a},$$

which cancels the dangerous coupling exactly.

This is the core “why tracking term is necessary” from the Lyapunov viewpoint.

2.4 Resulting contraction to an error ball (high-level inequality form)

After designing $\dot{\tilde{a}}$ and \dot{P} appropriately (next section), \dot{V} can be arranged into the form:

$$\dot{V} \leq -\alpha V + \beta,$$

with constants $\alpha > 0$ and $\beta \geq 0$ depending on:

- K (damping)
- boundedness of $d(t)$, measurement noise, and time-variation of $a(t)$

Solving the scalar differential inequality yields:

$$V(t) \leq e^{-\alpha t} V(0) + \frac{\beta}{\alpha} (1 - e^{-\alpha t}),$$

hence:

$$\limsup_{t \rightarrow \infty} V(t) \leq \frac{\beta}{\alpha},$$

which implies $[s; \tilde{a}]$ converges exponentially into a ball whose radius is proportional to $\sqrt{\beta/\alpha}$. This is the precise meaning of "equivalent energy shrinks to an error ball."

3. Optimal parameter estimation: obtain \hat{a} , \dot{P} and the gain (Kalman–Bucy structure)

3.1 Measurement and process models for the unknown coefficient $a(t)$

We assume we can form a (noisy) measurement $y(t) \in \mathbb{R}^n$ of the aerodynamic force component represented by ϕa

$$y(t) = \phi(q, \dot{q}) a(t) + \epsilon(t),$$

where $\epsilon(t)$ is measurement noise with covariance:

$$\mathbb{E}[\epsilon(t)\epsilon(\tau)^\top] = R\delta(t - \tau), \quad R \succ 0.$$

We also model the time-variation of $a(t)$ as a stable drift + process noise:

$$\dot{a}(t) = -\lambda a(t) + \nu(t),$$

with:

$$\mathbb{E}[\nu(t)\nu(\tau)^\top] = Q\delta(t - \tau), \quad Q \succeq 0.$$

Here:

- $\lambda \geq 0$ enforces "forgetting / leakage"
- Q encodes how fast we allow $a(t)$ to vary (wind variability)

3.2 Kalman–Bucy (continuous-time) estimator for $a(t)$

i. Stochastic formulation of the parameter–observation system

We consider an unknown scalar parameter $a(t)$ evolving in time and observed indirectly through noisy measurements. The deterministic rate equation

$$\dot{a}(t) = -\lambda a(t) + \nu(t)$$

is interpreted as a stochastic differential equation by modeling the uncertainty term $\nu(t)$ as white noise. Specifically, we write the parameter dynamics in Itô form as

$$da(t) = -\lambda a(t)dt + \sqrt{Q}dW_t$$

where W_t is a standard Brownian motion satisfying

$$\mathbb{E}[dW_t] = 0, \quad \mathbb{E}[(dW_t)^2] = dt$$

and $Q \geq 0$ represents the process noise intensity.

The observation model is given in algebraic form as

$$y(t) = \phi(t)a(t) + \epsilon(t)$$

where $\epsilon(t)$ is zero-mean measurement noise with variance $R > 0$. In continuous time, this is expressed in differential form as

$$dy(t) = \phi(t)a(t)dt + \sqrt{R}dV_t$$

where V_t is an independent standard Brownian motion with

$$\mathbb{E}[dV_t] = 0, \quad \mathbb{E}[(dV_t)^2] = dt$$

We assume W_t and V_t are independent.

ii Gaussianity of the stochastic processes

We assume a Gaussian prior for the initial parameter value,

$$a(0) \sim \mathcal{N}(\bar{a}_0, P_0).$$

Since the SDE for $a(t)$ is linear and driven by Gaussian noise, its explicit solution can be written as

$$a(t) = e^{-\lambda t}a(0) + \int_0^t e^{-\lambda(t-s)}\sqrt{Q}dW_s$$

Both terms on the right-hand side are linear functionals of Gaussian random variables; therefore $a(t)$ is Gaussian for all t

Similarly, the observation increment $dy(t)$ is a linear function of $a(t)$ plus Gaussian noise.

Hence, for any finite collection of times, the random variables

$$(a(t), y(t_1), \dots, y(t_n))$$

are jointly Gaussian.

Let $\mathcal{Y}_t := \sigma y(s) \mid 0 \leq s \leq t$ denote the observation history.

Then $a(t)$ and \mathcal{Y}_t are jointly Gaussian in the sense that all finite-dimensional distributions are jointly Gaussian.

iii Estimation objective and MMSE criterion

At time t , we seek an estimate of $a(t)$ using only the available observation history \mathcal{Y}_t .

Any admissible estimator must be of the form $\eta(\mathcal{Y}_t)$.

The estimation objective is to minimize the mean-square error

$$\mathbb{E}[(a(t) - \eta(\mathcal{Y}_t))^2]$$

This defines a projection problem in the Hilbert space $L^2(\Omega)$ of square-integrable random variables, equipped with the inner product

$$\langle X, Z \rangle := \mathbb{E}[XZ].$$

The set of all \mathcal{Y}_t -measurable random variables forms a closed linear subspace of $L^2(\Omega)$.

iv Orthogonal decomposition and Pythagorean identity

For any admissible estimator $\eta(\mathcal{Y}_t)$, we decompose the estimation error as

$$a(t) - \eta = (a(t) - \mathbb{E}[a(t) | \mathcal{Y}_t]) + (\mathbb{E}[a(t) | \mathcal{Y}_t] - \eta)$$

Squaring and taking expectations yields:

$$\begin{aligned} \mathbb{E}[(a - \eta)^2] &= \mathbb{E}[(a - \mathbb{E}[a | \mathcal{Y}_t])^2] + \mathbb{E}[(\mathbb{E}[a | \mathcal{Y}_t] - \eta)^2] \\ &\quad + 2\mathbb{E}[(a - \mathbb{E}[a | \mathcal{Y}_t])(\mathbb{E}[a | \mathcal{Y}_t] - \eta)] \end{aligned}$$

Using the tower property,

$$\mathbb{E}[Z] = \mathbb{E}[\mathbb{E}[Z | \mathcal{Y}_t]],$$

The cross term:

$$\mathbb{E}[(a - \mathbb{E}[a | \mathcal{Y}_t])(\mathbb{E}[a | \mathcal{Y}_t] - \eta)] = \mathbb{E}[\mathbb{E}[(a - \mathbb{E}[a | \mathcal{Y}_t])(\mathbb{E}[a | \mathcal{Y}_t] - \eta) | \mathcal{Y}_t]]$$

Given \mathcal{Y}_t , $\mathbb{E}[a | \mathcal{Y}_t] - \eta$ can be confirmed, and

$$\mathbb{E}[a - \mathbb{E}[a | \mathcal{Y}_t] | \mathcal{Y}_t] = 0$$

we obtain

$$\mathbb{E}[(a - \eta)^2] = \mathbb{E}[(a - \mathbb{E}[a | \mathcal{Y}_t])^2] + \mathbb{E}[(\mathbb{E}[a | \mathcal{Y}_t] - \eta)^2]$$

This is the Pythagorean identity in $L^2(\Omega)$.

v. Optimal estimator as conditional expectation

The first term in the above decomposition is independent of η , while the second term is nonnegative and vanishes if and only if

$$\eta(\mathcal{Y}_t) = \mathbb{E}[a(t) | \mathcal{Y}_t].$$

Therefore, the unique minimum-mean-square error (MMSE) estimator is

$$\hat{a}(t) = \mathbb{E}[a(t) | \mathcal{Y}_t]$$

This result does not rely on Gaussianity; it follows solely from the quadratic loss criterion and the geometry of $L^2(\Omega)$

To compute $\hat{a}(t)$ in continuous time, we exploit the fact that new information arrives through the observation increment $dy(t)$.

The observation history satisfies

$$\mathcal{Y}_{t+dt} = \sigma(\mathcal{Y}_t, dy(t))$$

By definition,

$$\hat{a}(t + dt) = \mathbb{E}[a(t + dt) | \mathcal{Y}_{t+dt}] = \mathbb{E}[a(t + dt) | \mathcal{Y}_t, dy(t)]$$

Writing $a(t + dt) = a(t) + da(t)$ and subtracting $\hat{a}(t)$, we obtain

$$d\hat{a} = \hat{a}(t + dt) - \hat{a}(t) = \mathbb{E}[a(t + dt) | \mathcal{Y}_t, dy(t)] - \mathbb{E}[a(t) | \mathcal{Y}_t]$$

$$\boxed{d\hat{a} = \mathbb{E}[da | \mathcal{Y}_t, dy] + (\mathbb{E}[a(t) | \mathcal{Y}_t, dy] - \mathbb{E}[a(t) | \mathcal{Y}_t])}$$

The first term represents the predicted drift of the estimate, while the second term represents the correction induced by the newly acquired observation increment.

Regardless of whether the condition is \mathcal{Y}_t or dy , the Brownian increment mean is 0.

$$\mathbb{E}[da \mid \mathcal{Y}_t, dy] = \mathbb{E}[-\lambda a(t)dt + \sqrt{Q}dW_t \mid \mathcal{Y}_t, dy] = -\lambda \mathbb{E}[a \mid \mathcal{Y}_t, dy]dt = -\lambda \hat{a}dt$$

By the joint Gaussian conditional mean formula,

$$\begin{aligned}\mathbb{E}[x \mid y] &= \mu_x + \Sigma_{xy} \Sigma_{yy}^{-1} (y - \mu_y) \\ \begin{pmatrix} x \\ y \end{pmatrix} &\sim \mathcal{N} \left(\begin{pmatrix} \mu_x \\ \mu_y \end{pmatrix}, \begin{pmatrix} \Sigma_{xx} & \Sigma_{xy} \\ \Sigma_{yx} & \Sigma_{yy} \end{pmatrix} \right) \\ \mathbb{E}[x \mid y] &= \mu_x + \frac{\text{Cov}(x, y)}{\text{Var}(y)} (y - \mu_y)\end{aligned}$$

Conditioned on \mathcal{Y}_t , the pair $(a(t), dy(t))$ is jointly Gaussian, since $dy(t)$ is a linear function of $a(t)$ plus Gaussian noise

$$a(t) \mid \mathcal{Y}_t \sim \text{Gaussian}$$

$$dy \mid \mathcal{Y}_t = \phi(t) a(t) dt + R^{1/2} dV_t, dV_t \sim \mathcal{N}(0, dt)$$

Hence, $(a(t), dy) \mid \mathcal{Y}_t$ is jointly Gaussian

$$\mu_a = \mathbb{E}[a(t) \mid \mathcal{Y}_t] = \hat{a}(t)$$

$$\mu_y = \mathbb{E}[dy \mid \mathcal{Y}_t]$$

$$P = \text{Var}(a(t) \mid \mathcal{Y}_t)$$

$$R = \text{Var}(dy \mid \mathcal{Y}_t)$$

$$C = \text{Cov}(a(t), dy \mid \mathcal{Y}_t)$$

$$\begin{pmatrix} a(t) \\ dy \end{pmatrix} \mid \mathcal{Y}_t \sim \mathcal{N} \left(\begin{pmatrix} \mu_a \\ \mu_y \end{pmatrix}, \begin{pmatrix} P & C \\ C^\top & R \end{pmatrix} \right)$$

$$\mathbb{E}[a(t) \mid \mathcal{Y}_t, dy] = \hat{a}(t) + \text{Cov}(a(t), dy \mid \mathcal{Y}_t) \text{Var}(dy \mid \mathcal{Y}_t)^{-1} (dy - \mathbb{E}[dy \mid \mathcal{Y}_t])$$

so,

$$\mathbb{E}[a(t) \mid \mathcal{Y}_t, dy] - \mathbb{E}[a(t) \mid \mathcal{Y}_t] = \text{Cov}(a(t), dy \mid \mathcal{Y}_t) \text{Var}(dy \mid \mathcal{Y}_t)^{-1} (dy - \mathbb{E}[dy \mid \mathcal{Y}_t])$$

Hence, the conditional expectation $\mathbb{E}[a(t) \mid \mathcal{Y}_t, dy]$ is linear in dy and can be expressed as a local regression on the innovation

$$d\nu(t) = dy(t) - \mathbb{E}[dy(t) \mid \mathcal{Y}_t] = dy(t) - \phi(t)\hat{a}(t)dt$$

This yields the continuous-time update structure for the optimal estimator.

Conditioned on \mathcal{Y}_t , Noise increment dV_t and $a(t)$ are independent, Calculate the two conditional covariances:

$$dy(t) = \phi(t)a(t)dt + \sqrt{R}dV_t$$

$$\boxed{\text{Cov}(a(t), dy \mid \mathcal{Y}_t) = \text{Cov}(a(t), \phi(t)a(t)dt \mid \mathcal{Y}_t) = \text{Cov}(a(t), a(t)dt \mid \mathcal{Y}_t)\phi(t)^\top = P(t)\phi(t)^\top dt}$$

where $P(t)dt = \text{Cov}(a(t), a(t)dt \mid \mathcal{Y}_t)$

$$\text{Cov}(a(t), a(t)dt \mid \mathcal{Y}_t) = dt \text{Cov}(a(t), a(t) \mid \mathcal{Y}_t) = dt \text{Var}(a(t) \mid \mathcal{Y}_t).$$

calculate $R = \text{Var}(dy \mid \mathcal{Y}_t)$

$$R = \text{Var}(dy \mid \mathcal{Y}_t) = \phi(t)a(t)dt + \sqrt{R}dV_t = Rdt + o(dt^2)$$

Finally, we obtain the differential of the \hat{d}

$$d\hat{a} = -\lambda\hat{a}dt + P(t)\phi(t)^\top dt(Rdt)^{-1}(dy(t) - \phi(t)\hat{a}(t)dt)$$

vi Define the mean-square estimation error and derive $\dot{P}(t)$

Define the estimation error

$$e(t) = a(t) - \hat{a}(t)$$

We define the (scalar) error mean-square as

$$P(t) = \mathbb{E}[e(t)^2 \mid \mathcal{Y}_t]$$

$$P(t) = \mathbb{E}[e(t)^2 \mid \mathcal{Y}_t] = \text{Var}(a(t) \mid \mathcal{Y}_t).$$

(Equivalently, one may use the conditional version $P(t) := \mathbb{E}[e(t)^2 \mid \mathcal{Y}_t]$; in the linear-Gaussian setting this $P(t)$ turns out to be deterministic and satisfies the same Riccati ODE.

$$de(t) = da(t) - d\hat{a}(t)$$

$$e_y(t) = y(t) - \phi(t)\hat{a}(t).$$

$$dy(t) = \phi(t)a(t)dt + \sqrt{R}dV_t$$

Substitute the expressions above:

$$de(t) = \left(-\lambda a(t)dt + \sqrt{Q}dW_t \right) - \left(-\lambda \hat{a}(t)dt + K(t)(dy(t) - \phi(t)\hat{a}(t)dt) \right)$$

Group terms. First the drift terms:

$$-\lambda a(t)dt + \lambda \hat{a}(t)dt = -\lambda(a(t) - \hat{a}(t))dt = -\lambda e(t)dt$$

Then the correction drift:

$$-K(t)(dy(t) - \phi(t)\hat{a}(t)dt) = -K(t)(\phi(t)a(t)dt + \sqrt{R}dV_t - \phi(t)\hat{a}(t)dt) = -K(t)\phi(t)e(t)dt - K(t)\sqrt{R}dV_t$$

Therefore the error SDE is

$$de(t) = -(\lambda + K(t)\phi(t))e(t)dt + \sqrt{Q}dW_t - K(t)\sqrt{R}dV_t$$

$$d(e^2) = 2ede + (de)^2$$

The term $2ede$. Using the error SDE,

$$2ede = 2e \left(-(\lambda + K\phi)e dt + \sqrt{Q}dW_t - K\sqrt{R}dV_t \right) = -2(\lambda + K\phi)e^2 dt + 2e\sqrt{Q}dW_t - 2eK\sqrt{R}dV_t$$

The quadratic variation term $(de)^2$. Since dt is higher order compared to Brownian increments, we keep only the dW_t and dV_t parts:

$$de = \dots + \sqrt{Q}dW_t - K\sqrt{R}dV_t$$

Thus,

$$(de)^2 = (\sqrt{Q}dW_t - K\sqrt{R}dV_t)^2 = Q(dW_t)^2 - 2K\sqrt{QR}dW_t dV_t + K^2 R(dV_t)^2$$

Using independence of W_t and V_t ,

$$dW_t dV_t = 0$$

and the Itô identities

$$(dW_t)^2 = dt, \quad (dV_t)^2 = dt$$

we obtain

$$(de)^2 = (Q + K^2 R)dt$$

$$\boxed{d(e^2) = -2(\lambda + K\phi)e^2 dt + (Q + K^2 R)dt + 2e\sqrt{Q}dW_t - 2eK\sqrt{R}dV_t}$$

Recall $P(t) = \mathbb{E}[e(t)^2]$. Taking expectation on both sides:

$$d\mathbb{E}[e^2] = \mathbb{E}[d(e^2)]$$

Now use the fact that Itô integrals have zero mean (under standard integrability conditions):

$$\mathbb{E}[e(t)dW_t] = 0, \quad \mathbb{E}[e(t)dV_t] = 0.$$

Hence the stochastic terms vanish in expectation, yielding

$$dP(t) = \left(-2(\lambda + K(t)\phi(t))\mathbb{E}[e(t)^2] + Q + K(t)^2 R \right) dt$$

$$\dot{P}(t) = -2(\lambda + K(t)\phi(t))P(t) + Q + K(t)^2 R.$$

For the linear-Gaussian MMSE filter, the gain is

$$K(t) = \frac{P(t)\phi(t)}{R}.$$

Substitute into the ODE:

$$\dot{P}(t) = -2\lambda P(t) - 2\left(\frac{P(t)\phi(t)}{R}\right)\phi(t)P(t) + Q + \left(\frac{P(t)\phi(t)}{R}\right)^2 R.$$

Compute each term carefully:

The middle drift correction term:

$$-2\left(\frac{P\phi}{R}\right)\phi P = -\frac{2\phi(t)^2}{R}P(t)^2$$

The last term:

$$\left(\frac{P\phi}{R}\right)^2 R = \frac{\phi(t)^2}{R}P(t)^2$$

Combine them:

$$-\frac{2\phi(t)^2}{R}P(t)^2 + \frac{\phi(t)^2}{R}P(t)^2 = -\frac{\phi(t)^2}{R}P(t)^2$$

Therefore the final Riccati equation for the mean-square estimation error is

$$\boxed{\dot{P}(t) = -2\lambda P(t) + Q - \frac{\phi(t)^2}{R}P(t)^2.}$$

This equation shows explicitly how the uncertainty evolves:

- $-2\lambda P$ comes from the stable drift $-\lambda a$ (forgetting/decay of uncertainty),
- $+Q$ comes from process noise injection
- $-(\phi^2/R)P^2$ is the information gain from measurements (stronger sensing ϕ or smaller noise R reduces P faster).

vii Matrix generalization

Now let:

$$a(t) \in \mathbb{R}^h, \quad \hat{a}(t) \in \mathbb{R}^h, \quad \tilde{a} = \hat{a} - a \in \mathbb{R}^h,$$

$$\text{and measurement: } y(t) \in \mathbb{R}^n, \quad y = \phi a + \epsilon, \quad \phi \in \mathbb{R}^{n \times h}.$$

Noise covariances:

$$\mathbb{E}[\epsilon\epsilon^\top] = R, \quad R \in \mathbb{R}^{n \times n}, \quad R \succ 0, \quad \mathbb{E}[\nu\nu^\top] = Q, \quad Q \in \mathbb{R}^{h \times h}, \quad Q \succeq 0.$$

The continuous-time Kalman-Bucy estimator has the form:

$$\dot{\hat{a}} = -\lambda \hat{a} + P\phi^\top R^{-1}(y - \phi \hat{a})$$

and the covariance evolution becomes the matrix Riccati equation:

$$\dot{P} = -2\lambda P + Q - P\phi^\top R^{-1}\phi P.$$

The matrix Kalman gain is:

$$K_a(t) = P(t)\phi(t)^\top R^{-1}.$$

In our composite adaptation law, we will then add the tracking-driven term:

$$\dot{\hat{a}} = -\lambda \hat{a} + P\phi^\top R^{-1}(y - \phi \hat{a}) + P\phi^\top s.$$